AES/Vec.lean
@@ -22,11 +22,12 @@ instance [DecidableEq α] : DecidableEq (Vec n α) :=
     | isTrue h  => isTrue (eq_of_val_eq h)
     | isFalse h => isFalse (ne_of_val_ne h)
 
-def mkEmpty (n : Nat) : Vec 0 α := { value := .mkEmpty n, sizeEq := rfl }
-
 def cast : n = m → Vec n α → Vec m α | rfl, x => x
 
+def mkEmpty (n : Nat) : Vec 0 α := { value := .mkEmpty n, sizeEq := rfl }
+
 def empty : Vec 0 α := mkEmpty 0
+
 
 def push (v : Vec n α) (a : α) : Vec (n + 1) α :=
   { value := v.value.push a,
@@ -54,6 +55,63 @@ instance : GetElem (Vec n α) (Fin n) α (fun _ _ => True) where
 instance : GetElem (Vec n α) Nat α (fun _ i => i < n) where
   getElem v i p := v.get ⟨i, p⟩
 
+
+@[simp] theorem castGetElem : ∀(v : Vec m α) (g : m = n) (i : Nat) (h : i < n),
+      (cast g v)[i]'h = v[i]'(by simp [g, h])
+  | _, rfl, _, _ => rfl
+
+
+@[simp] theorem pushGetElem (v : Vec n α) (a : α) (i : Nat) (h : i < n + 1) :
+    (v.push a)[i]'h = if p : i < n then v[i]'p else a := by
+  unfold push
+  simp [GetElem.getElem]
+  unfold Vec.get
+  if p : i < n then
+    simp [p, Vec.sizeEq, Array.get_push_lt]
+  else
+    have q : i = v.value.size := by
+      simp [Vec.sizeEq];
+      omega
+    simp only [p, dite_false]
+    simp [q, Array.get_push_eq]
+
+theorem getElemOfFn (f : Fin n → α) (i : Nat) (h : i < n) :
+    (Vec.ofFn f)[i]'h = f ⟨i, h⟩ := by
+  unfold Vec.ofFn
+  let rec auxP {m : Nat} (a : Vec m α) (p : m ≤ n) : (ofFnAux f a p)[i] =
+          if q : i < m then a[i]'q else f ⟨i, h⟩ := by
+    unfold ofFnAux
+    if lt : m < n then
+      simp [lt, auxP (a.push _)]
+      match Nat.lt_trichotomy i m with
+      | Or.inl q =>
+        simp [q, Nat.lt_succ_of_lt q]
+      | Or.inr (Or.inl q) =>
+        simp [q]
+      | Or.inr (Or.inr q) =>
+        have q2 : ¬(i < m + 1) := by omega
+        have q3 : ¬(i < m) := by omega
+        simp [q2, q3]
+    else
+      have q2 : i < m := by omega
+      simp [lt, q2]
+    termination_by n - m
+  simp [auxP]
+  intro q
+  contradiction
+
+theorem valueGetElem (x : Vec n α) (i : Nat) (h : i < x.value.size) :
+    x.value[i]'h = x[i]'(by simp [x.sizeEq] at h; exact h) := by
+  rfl
+
+def ext {x y : Vec n α} (p : ∀(i : Fin n), x[i] = y[i]) : x = y := by
+  apply eq_of_val_eq
+  apply Array.ext
+  · simp [Vec.sizeEq]
+  intros i ltx lty
+  simp only [valueGetElem]
+  exact p ..
+
 protected def map (f : α → β) (x : Vec n α) : Vec n β := .ofFn (fun i => f x[i])
 
 instance : Functor (Vec n) where
@@ -61,6 +119,9 @@ instance : Functor (Vec n) where
 
 def ofList (l : List α) : Vec l.length α := { value := l.toArray, sizeEq := Array.size_toArray l }
 
+/--
+Rotate value to left if `i` is positive and to right if negative.
+-/
 def rotate (x : Vec n α) (i : Int) : Vec n α := .ofFn fun j =>
   let idx := ((j.val + i)%n).toNat
   let p : idx < n := by
@@ -131,6 +192,7 @@ def mkVecExpr (nExpr : Expr) : MetaM (Level × Expr × Expr) := do
 
 elab_rules : term <= ptp
   | `(#v[ $elems,* ]) => do
+
     let a := elems.getElems
     let n := a.size
     let rnExpr <- freshNatExpr
@@ -145,6 +207,8 @@ elab_rules : term <= ptp
             let v' := mkApp4 (.const ``Vec.push [lvl]) (toExpr n) etp v e
             pure (v', n + 1)
       let (v, _) <- a.foldlM (init := (empty, 0)) pushVal
+--      unless (← isDefEq rnExpr (natExpr n)) do
+--        logError "bad"
       pure v
     else
       throwError m!"Expected vector instead of {ptp}"
